add a simp attribute `tl_simp` to use in `[temporal]` mode. This is an attempt at improving the performances of temporal proofs

src/collate.hs
@@ -1,0 +1,64 @@
+{-# LANGUAGE LambdaCase #-}
+
+module Main where
+
+import Control.Monad
+import Data.Bifunctor
+import Data.Maybe
+import qualified Data.Map as M
+import Data.List
+import System.IO
+import Text.Printf
+
+import Pipes
+import qualified Pipes.Prelude as P
+
+inputFile :: String
+inputFile = "report.txt"
+
+compileTimestamp :: [String] -> Maybe (String,Int)
+compileTimestamp [_,t,_,fn] = Just (fn,read $ take (length t - 2) t)
+compileTimestamp _ = Nothing
+
+takeWhile' :: ([a] -> Bool) -> [a] -> [a]
+takeWhile' _ [] = []
+takeWhile' p (x:xs) | p (x:xs)  = x : takeWhile' p xs
+                    | otherwise = []
+
+compileTimestamp' :: [String] -> Maybe (String,Int)
+compileTimestamp' [_,t,_,fn] = Just (takeWhile' (not . isPrefixOf "._") fn,read $ take (length t - 2) t)
+compileTimestamp' _ = Nothing
+
+-- grep -R . -e "% *temporal\\." --include ".*\\.out" > report.txt
+
+data Cell = LeftAlign String | RightAlign String
+
+render :: Int -> Cell -> String
+render w (LeftAlign out)  = out ++ replicate (w - length out) ' '
+render w (RightAlign out) = replicate (w - length out) ' ' ++ out
+
+size :: Cell -> Int
+size (LeftAlign out)  = length out
+size (RightAlign out) = length out
+
+mkTable :: [Maybe (Cell,Cell)] -> Producer String IO ()
+mkTable rows = do
+  let m0 = maximum (mapMaybe (fmap $ size . fst) rows)
+      m1 = maximum (mapMaybe (fmap $ size . snd) rows)
+  yield $ printf "+%s+%s+" (replicate (m0 + 2) '-') (replicate (m1 + 2) '-')
+  forM_ rows $ \case
+    Just (x,y) -> yield $ printf "| %s | %s |" (render m0 x) (render m1 y)
+    Nothing    -> yield $ printf "+%s+%s+" (replicate (m0 + 2) '-') (replicate (m1 + 2) '-')
+  yield $ printf "+%s+%s+" (replicate (m0 + 2) '-') (replicate (m1 + 2) '-')
+
+
+main :: IO ()
+main = do
+  lns <- lines <$> readFile inputFile
+  let ls = mapMaybe (compileTimestamp' . words) lns
+  let m = M.fromListWith (+) ls
+  let result = take 40 $ reverse $ sortOn snd $ M.toList m
+      heading = Just (LeftAlign "function",LeftAlign "total time (ms)")
+      table = heading : Nothing : map (Just . bimap LeftAlign (RightAlign . show)) result
+  withFile "result.org" WriteMode $ \h ->
+    runEffect $ mkTable table >-> P.toHandle h
