src/temporal_logic/spec.lean
@@ -12,21 +12,21 @@ variables (p : pred' α)
 variables (cs fs : evt → pred' α)
 variables (A : evt → act α)
 
-@[simp]
+@[simp, tl_simp]
 def spec_saf_spec (v : tvar α) (sch : tvar evt) : cpred :=
 p ! v ⋀
 ◻(∃∃ e, sch ≃ ↑e ⋀ cs e ! v ⋀ fs e ! v ⋀ ⟦ v | A e ⟧)
 
-@[simp]
+@[simp, tl_simp]
 def spec (v : tvar α) : cpred :=
 p ! v ⋀
 ◻(∃∃ e, cs e ! v ⋀ fs e ! v ⋀ ⟦ v | A e ⟧) ⋀
 ∀∀ e, sched (cs e ! v) (fs e ! v) ⟦ v | A e ⟧
 
-@[simp]
+@[simp, tl_simp]
 def spec_sch (v : tvar α) (sch : tvar evt) : cpred :=
 p ! v ⋀
-◻(∃∃ e, sch ≃ ↑e ⋀ cs e ! v ⋀ fs e ! v ⋀ ⟦ v | A e ⟧) ⋀
+◻(∃∃ e, sch ≃ ↑e ⋀ cs e!v ⋀ fs e!v ⋀ ⟦ v | A e ⟧) ⋀
 ∀∀ e, sched (cs e ! v) (fs e ! v) (sch ≃ e ⋀ ⟦ v | A e ⟧)
 
 
